```

x1, x2, ..., xn

Given n integers

Each time we can produce 2x - y, x and y can be any integers we have previously


Claim : From any integer x[i], we can reach x[i] +- k|x[i]-x[j]|

Let a = x[i], b = x[j]


2x - y = 2a - b = a + (a-b)

If a > b, we're basically getting the reflection of b over a

b----a----(a + (a-b))

Imaigne b and a on a number line, by doing 2a-b, we get b on the other side of a.

We can do the above to basically get any a + k|a-b|.

So the above is proven,

(From editorial)

now let x1 = 0, if x1 != 0, we can just subtract everything by x1 including k. This wouldn't really change anything, cus we shifted all the value together. Difference between every elements still stay the same.

We will now prove that the answer is "YES" if and only if k can be divided by g=gcd(x2,x3,…,xn).

Every number produced is divisible by g, this is because g | x, g | y which implied g | 2x - y

Now to prove that for any x divisible by g we can write it on the board.

For the case when we just have 

(0, a) it is pretty obvious, as we have shown in the above.

But what about the case where we have more numbers? Notice that we just need to retrieve g=gcd(x2,x3,…,xn) and we will basically have (0,g) pair.

But what guarantees us that we can get g?

Let's prove this using induction,

Assume we can get g0 = gcd(x2,x3...,xn-1),

By Bezout's Theorem / Extended GCD, we know that there exists integer a, b s.t ax + by = gcd(x,y)

So as we have g0 and xn in the array now. By Bezout's Theorem, we know that we can also get g = gcd(g0, xn)

Let's further show it,

The equation we have is 2x-y,

For the equation, ax + by, let's substite g0 and xn, so we will have

a(g0) + b(xn)

From the above we know that, we can generate any a(g0), and any b(xn) individually. 

We just need to find such pair s.t either a or b is even and that will produce g when a(g0) + b(xn).

Without loss of generality, let's assume b is even, let it be 2k.

So we will have a(g0) + (2k)(xn) = 2k(xn) + a(g0),

this equation can easily be substituted into 2x - y. 

with k(xn) and a(g0), and we can retrieve g from here.

But what if none of them is even?

Well that would not be the case, because let's say a and b is both an odd number, let x' = g0/g, y' = xn/g, x' and y' are coprime, so they cannot be even.

We can find another solution (because its not unique, for more about this, look up diophatine equation) for this.

a = a+y' 
b = b-x'

odd+odd, odd-odd will give even, so all good :)

Useful links :
https://codeforces.com/blog/entry/87294 (The editorial)
https://codeforces.com/blog/entry/87294?#comment-755019 (How to apply berzout identity with the equation 2x-y)
https://codeforces.com/blog/entry/87294?#comment-754746 (What if coefficients of bezout identity are both odd?)
```
```cpp

#include <bits/stdc++.h>
#define all(x) begin(x),end(x)
#define fir first
#define sec second
#define sz(x) x.size()
#define pb push_back
 
using namespace std;
using ll = long long;
using vi = vector<int>;
using pi = pair<int,int>;
using pdb = pair<double,double>;
using pll = pair<ll,ll>;
using vll = vector<ll>;
using ull = unsigned long long;
const double EPS = (1e-6);
 
void setio(string s){
    freopen((s + ".in").c_str(),"r",stdin);
    freopen((s + ".out").c_str(),"w",stdout);
}

ll gcd(ll a, ll b){
    return (!b ? a : gcd(b, a % b));
}

void solve(){
    ll n, k;
    cin >> n >> k;

    vll a(n);
    for(auto& i : a) cin >> i;

    ll first = a[0];
    for(int i{}; i < n; i++){
        a[i] -= first;
    }

    k -= first;

    ll g = a[0];
    for(int i{}; i < n; i++){
        g = gcd(g, a[i]);
    }

    cout << (k % g == 0 ? "YES" : "NO") << '\n';
}

int main(){
    ios_base::sync_with_stdio(false);
    cin.tie(nullptr);
    int t = 1;
    cin >> t;
    while(t--){
        solve();
    }
    return 0;
}
 



```